transforms.v
@@ -1,4 +1,5 @@
 (** * Transform Language *)
+
 Set Warnings "-notation-overridden,-parsing".
 From LF Require Import imports.
 
@@ -14,6 +15,10 @@ Inductive AbBinExpr : Type :=
   | BinTrue
   | BinFalse.
 
+Inductive AbCommand : Type :=
+  | AbSkip
+  | AbAssign (x : string) (a : AbNumExpr).
+
 Fixpoint AbEval (st : state) (a : AbNumExpr) : nat :=
   match a with
   | AbLit l => l
@@ -26,6 +31,10 @@ Fixpoint AbBinEval (st : state) (b : AbBinExpr) : bool :=
   | BinFalse    => false
   end.
 
-Inductive AbCommand : Type :=
-  | AbSkip
-  | AbAssign (x : string) (a : AbNumExpr).
+Inductive AbExec : AbCommand -> state -> state -> Prop :=
+  | Ab_Skip : forall st,
+      AbSkip / st \\ st
+  | Ab_Assign  : forall st a1 n x,
+      AbEval st a1 = n ->
+      (AbAssign x a1) / st \\ st & { x --> n }
+  where "c1 '/' st '\\' st'" := (AbExec c1 st st').
